Membership in candidates preserved under evaluation

formal/SkLean/Sn.lean
@@ -38,13 +38,12 @@ lemma is_value_sn (h_v : is_value e) : sn e := by
   repeat do_stuck
 
 inductive is_candidate_for_ty : Expr → Expr → Prop
-  | val : valid_judgment e t
+  | val  : valid_judgment e t
     → is_value e
     → is_candidate_for_ty e t
-  | app : is_candidate_for_ty lhs SKM[(t_in ~> t_out)]
-    → is_candidate_for_ty rhs t_out
-    → (∀ e', is_eval_once SKM[(lhs rhs)] e' → is_candidate_for_ty e' t_out)
-    → is_candidate_for_ty SKM[(lhs rhs)] t_out
+  | step : valid_judgment e t
+    → (∀ e', is_eval_once e e' → is_candidate_for_ty e' t)
+    → is_candidate_for_ty e t
 
 namespace is_candidate_for_ty
 
@@ -54,15 +53,37 @@ lemma all_sn (h_candidate : is_candidate_for_ty e t) : sn e := by
   apply sn.intro
   assumption
 
-lemma all_well_typed (h_candidate : is_candidate_for_ty e t) : valid_judgment_hard e t := by
+lemma all_well_typed (h_candidate : is_candidate_for_ty e t) : valid_judgment e t := by
   induction h_candidate
-  
+  repeat assumption
+
+lemma preserved (h_candidate : is_candidate_for_ty e t) (h_step : is_eval_once e e') : is_candidate_for_ty e' t := by
+  let h_t := h_candidate.all_well_typed
+  induction h_candidate
+  case val e'' t' h_t h_val =>
+    have h := h_val.no_step
+    simp_all
+  case step e'' t' h_t ih₁ ih₂ =>
+    exact ih₁ _ h_step
 
 end is_candidate_for_ty
 
 namespace valid_judgment
 
-
+lemma all_candidates (h : valid_judgment e t) : is_candidate_for_ty e t := by
+  have h_progress := h.progress
+  match h_progress with
+    | .inl h_stuck =>
+      exact is_candidate_for_ty.val h h_stuck
+    | .inr ⟨e', h_step⟩ =>
+      have h_preservation := h.preservation h_step
+      induction h generalizing e'
+      repeat contradiction
+      apply is_candidate_for_ty.step
+      apply valid_judgment.call
+      repeat assumption
+      intro e'' h_step'
+      
 
 end valid_judgment
 
